problemaBancnotelor.dfy
@@ -1,173 +1,184 @@
 predicate esteSolutieValida(solutie : seq<int>)
 {
-  |solutie| == 4 && solutie[0]>=0 && solutie[1]>=0 && solutie[2]>=0 && solutie[3]>=0
+  |solutie| == 5 && solutie[0] >= 0 && solutie[1] >= 0 && solutie[2] >= 0 && solutie[3] >=0 && solutie[4] >=0
 }
 
-
-
-predicate esteSolutie(solutie : seq<int>, nr:int)
+predicate esteSolutie(solutie : seq<int>, suma : int)
   requires esteSolutieValida(solutie)
 {
-    solutie[0]*1+solutie[1]*5+solutie[2]*10+solutie[3]*20 == nr
+    solutie[0] * 1 + solutie[1] * 5 + solutie[2] * 10 + solutie[3] * 20 + solutie[4] * 50 == suma
 
 }
 
 
-function cost(solutie : seq<int>):int 
+function cost(solutie : seq<int>) : int 
   requires esteSolutieValida(solutie)
 {
-    solutie[0]+solutie[1]+solutie[2]+solutie[3]
+    solutie[0] + solutie[1] + solutie[2] + solutie[3] + solutie[4]
 }
 
-predicate esteSolutieOptima(solutie : seq<int>, nr:int)
+predicate esteSolutieOptima(solutie : seq<int>, suma : int)
     requires esteSolutieValida(solutie)
 {   
-  esteSolutie(solutie,nr) &&
-  forall solutieOarecare :: esteSolutieValida(solutieOarecare) && esteSolutie(solutieOarecare,nr) 
+  esteSolutie(solutie, suma) &&
+  forall solutieOarecare :: esteSolutieValida(solutieOarecare) && esteSolutie(solutieOarecare, suma) 
           ==> cost(solutieOarecare) >= cost(solutie)
 
 }
 
-predicate INV(copie: int, nr: int, solutieFinala : seq<int>)
+predicate INV(rest : int, suma : int, solutieFinala : seq<int>)
   requires esteSolutieValida(solutieFinala)
 {
    forall solutieCurenta :: esteSolutieValida(solutieCurenta) ==>
-          (esteSolutie(solutieCurenta,copie) ==> 
-          esteSolutie([solutieFinala[0]+solutieCurenta[0],solutieFinala[1]+solutieCurenta[1],
-          solutieFinala[2]+solutieCurenta[2],solutieFinala[3]+solutieCurenta[3]],nr)) &&
-          (esteSolutieOptima(solutieCurenta,copie) ==> 
-          esteSolutieOptima([solutieFinala[0]+solutieCurenta[0],solutieFinala[1]+solutieCurenta[1],
-          solutieFinala[2]+solutieCurenta[2],solutieFinala[3]+solutieCurenta[3]],nr))
+          (esteSolutie(solutieCurenta, rest) ==> 
+          esteSolutie([solutieFinala[0] + solutieCurenta[0], solutieFinala[1] + solutieCurenta[1], 
+          solutieFinala[2] + solutieCurenta[2], solutieFinala[3] + solutieCurenta[3], solutieFinala[4] + solutieCurenta[4]], suma)) &&
+          (esteSolutieOptima(solutieCurenta, rest) ==> 
+          esteSolutieOptima([solutieFinala[0] + solutieCurenta[0], solutieFinala[1] + solutieCurenta[1],
+          solutieFinala[2] + solutieCurenta[2], solutieFinala[3] + solutieCurenta[3], solutieFinala[4] + solutieCurenta[4]], suma))
 }
 
 
-method gasireMaxim(nr: int) returns(s:int)
-  requires nr > 0
-  ensures 0 < s <= nr
-  ensures s == 1 || s == 5 || s == 10 || s == 20
-  ensures s == 1 ==> nr < 5
-  ensures s == 5 ==> 5 <= nr < 10
-  ensures s == 10 ==> 10 <= nr < 20
-  ensures s == 20 ==> nr >= 20
+method gasireMaxim(suma : int) returns(s : int)
+  requires suma > 0
+  ensures 0 < s <= suma
+  ensures s == 1 || s == 5 || s == 10 || s == 20 || s == 50
+  ensures s == 1 ==> suma < 5
+  ensures s == 5 ==> 5 <= suma < 10
+  ensures s == 10 ==> 10 <= suma < 20
+  ensures s == 20 ==> 20 <= suma < 50
+  ensures s == 50 ==> suma >= 50
 {
-    if(nr >= 20)
+    if(suma >= 50)
+    {
+        s := 50 ;
+    }
+    else if(suma >= 20)
     {
         s := 20;
     }
-    else if(nr >= 10){
+    else if(suma >= 10)
+    {
         s := 10;
-        }
-        else if(nr >= 5){
+    }
+    else if(suma >= 5)
+    {
         s := 5;
-            }
-            else if(nr < 5){
-                s := 1; 
-            }
+    }
+    else if(suma < 5){
+        s := 1; 
+    }
 
 }
 
 
-lemma cazMaxim1(copie: int, nr: int, solutieFinala: seq<int>)
-  requires copie < 5
+lemma cazMaxim1(rest : int, suma : int, solutieFinala : seq<int>)
+  requires rest < 5
   requires esteSolutieValida(solutieFinala)
-  requires INV(copie,nr,solutieFinala)
-  ensures INV(copie-1,nr,[(solutieFinala[0]+1),solutieFinala[1],solutieFinala[2],solutieFinala[3]])
+  requires INV(rest, suma, solutieFinala)
+  ensures INV(rest-1, suma, [solutieFinala[0] + 1, solutieFinala[1], solutieFinala[2], solutieFinala[3], solutieFinala[4]])
 {
 
-  forall solutieCurenta | esteSolutieValida(solutieCurenta) && esteSolutieOptima(solutieCurenta,copie-1) 
-          ensures esteSolutieOptima([solutieFinala[0]+solutieCurenta[0]+1,solutieFinala[1]+solutieCurenta[1],
-          solutieFinala[2]+solutieCurenta[2],solutieFinala[3]+solutieCurenta[3]],nr)
+  forall solutieCurenta | esteSolutieValida(solutieCurenta) && esteSolutieOptima(solutieCurenta, rest - 1) 
+          ensures esteSolutieOptima([solutieFinala[0] + solutieCurenta[0] + 1, solutieFinala[1] + solutieCurenta[1],
+          solutieFinala[2] + solutieCurenta[2], solutieFinala[3] + solutieCurenta[3], solutieFinala[4] + solutieCurenta[4]], suma)
   {
-    assert esteSolutie(solutieCurenta,copie-1);
-    assert esteSolutie([solutieCurenta[0]+1,solutieCurenta[1],solutieCurenta[2],solutieCurenta[3]],copie);
+    assert esteSolutie(solutieCurenta, rest - 1);
+    assert esteSolutie([solutieCurenta[0] + 1, solutieCurenta[1], solutieCurenta[2], solutieCurenta[3], solutieCurenta[4]], rest);
 
-    assert forall solutieOarecare :: esteSolutieValida(solutieOarecare) && esteSolutie(solutieOarecare,copie-1) 
+    assert forall solutieOarecare :: esteSolutieValida(solutieOarecare) && esteSolutie(solutieOarecare, rest - 1) 
           ==> cost(solutieOarecare) >= cost(solutieCurenta);
 
-    assert esteSolutie([solutieFinala[0]+solutieCurenta[0]+1,solutieFinala[1]+solutieCurenta[1],
-          solutieFinala[2]+solutieCurenta[2],solutieFinala[3]+solutieCurenta[3]],nr);
+    assert esteSolutie([solutieFinala[0] + solutieCurenta[0] + 1, solutieFinala[1] + solutieCurenta[1],
+          solutieFinala[2] + solutieCurenta[2], solutieFinala[3] + solutieCurenta[3], solutieFinala[4] + solutieCurenta[4]], suma);
 
-    assert forall solutieOarecare :: esteSolutieValida(solutieOarecare) &&  esteSolutie(solutieOarecare,nr) 
-          ==> cost(solutieOarecare) >= cost([solutieCurenta[0]+solutieFinala[0]+1,solutieCurenta[1]+solutieFinala[1],
-          solutieCurenta[2]+solutieFinala[2],solutieCurenta[3]+solutieFinala[3]]);
+    assert forall solutieOarecare :: esteSolutieValida(solutieOarecare) &&  esteSolutie(solutieOarecare, suma) 
+          ==> cost(solutieOarecare) >= cost([solutieCurenta[0] + solutieFinala[0] + 1, solutieCurenta[1] + solutieFinala[1],
+          solutieCurenta[2] + solutieFinala[2], solutieCurenta[3] + solutieFinala[3], solutieCurenta[4] + solutieFinala[4]]);
   }
 
   assert forall solutieCurenta :: esteSolutieValida(solutieCurenta) 
-          && esteSolutieOptima(solutieCurenta,copie-1) ==> 
-          esteSolutieOptima([solutieFinala[0]+solutieCurenta[0]+1,solutieFinala[1]+solutieCurenta[1],
-          solutieFinala[2]+solutieCurenta[2],solutieFinala[3]+solutieCurenta[3]],nr);
-
+          && esteSolutieOptima(solutieCurenta, rest - 1) ==> 
+          esteSolutieOptima([solutieFinala[0] + solutieCurenta[0] + 1, solutieFinala[1] + solutieCurenta[1],
+          solutieFinala[2] + solutieCurenta[2], solutieFinala[3] + solutieCurenta[3], solutieFinala[4] + solutieCurenta[4]], suma);
 }
 
-lemma cazMaxim5(copie: int, nr: int, solutieFinala: seq<int>)
-  requires 5 <= copie < 10 
+lemma cazMaxim5(rest : int, suma : int, solutieFinala : seq<int>)
+  requires 5 <= rest < 10 
   requires esteSolutieValida(solutieFinala)
-  requires INV(copie,nr,solutieFinala)
-  ensures INV(copie-5,nr,[solutieFinala[0],(solutieFinala[1]+1),solutieFinala[2],solutieFinala[3]])
+  requires INV(rest, suma, solutieFinala)
+  ensures INV(rest - 5, suma, [solutieFinala[0], solutieFinala[1] + 1, solutieFinala[2], solutieFinala[3], solutieFinala[4]])
 {
 
- forall solutieCurenta | esteSolutieValida(solutieCurenta) && esteSolutieOptima(solutieCurenta,copie-5) 
-          ensures esteSolutieOptima([solutieFinala[0]+solutieCurenta[0],solutieFinala[1]+solutieCurenta[1]+1,
-          solutieCurenta[2]+solutieFinala[2],solutieCurenta[3]+solutieFinala[3]],nr)
+ forall solutieCurenta | esteSolutieValida(solutieCurenta) && esteSolutieOptima(solutieCurenta, rest - 5) 
+          ensures esteSolutieOptima([solutieFinala[0] + solutieCurenta[0], solutieFinala[1] + solutieCurenta[1] + 1,
+          solutieCurenta[2] + solutieFinala[2], solutieCurenta[3] + solutieFinala[3], solutieFinala[4]], suma)
   {
-    assert esteSolutie(solutieCurenta,copie-5);
-    assert esteSolutie([solutieCurenta[0], solutieCurenta[1]+1,solutieCurenta[2],solutieCurenta[3]],copie);
+    assert esteSolutie(solutieCurenta, rest - 5);
+    assert esteSolutie([solutieCurenta[0], solutieCurenta[1] + 1, solutieCurenta[2], solutieCurenta[3], solutieCurenta[4]], rest);
 
-    assert forall solutieOarecare :: esteSolutieValida(solutieOarecare)  && esteSolutie(solutieOarecare,copie-5) 
+    assert forall solutieOarecare :: esteSolutieValida(solutieOarecare)  && esteSolutie(solutieOarecare, rest - 5) 
           ==> cost(solutieOarecare) >= cost(solutieCurenta);
-    assert esteSolutie([solutieFinala[0]+solutieCurenta[0],solutieFinala[1]+solutieCurenta[1]+1,solutieFinala[2]+solutieCurenta[2],solutieFinala[3]+solutieCurenta[3]],nr);
+    assert esteSolutie([solutieFinala[0] + solutieCurenta[0], solutieFinala[1] + solutieCurenta[1] + 1,
+            solutieFinala[2] + solutieCurenta[2], solutieFinala[3] + solutieCurenta[3], solutieFinala[4] + solutieCurenta[4]], suma);
     
-    assert forall solutieOarecare :: esteSolutieValida(solutieOarecare) && esteSolutie(solutieOarecare,nr)
-          ==> cost(solutieOarecare) >= cost([solutieFinala[0]+solutieCurenta[0],solutieFinala[1]+solutieCurenta[1]+1,solutieFinala[2]+solutieCurenta[2],solutieFinala[3]+solutieCurenta[3]]);
+    assert forall solutieOarecare :: esteSolutieValida(solutieOarecare) && esteSolutie(solutieOarecare, suma)
+          ==> cost(solutieOarecare) >= cost([solutieFinala[0] + solutieCurenta[0], solutieFinala[1] + solutieCurenta[1] + 1,
+          solutieFinala[2] + solutieCurenta[2], solutieFinala[3] + solutieCurenta[3], solutieFinala[4] + solutieCurenta[4]]);
   }
 
-  assert forall solutieCurenta :: esteSolutieValida(solutieCurenta) && esteSolutie(solutieCurenta,copie-5) ==> 
-          esteSolutieOptima([solutieCurenta[0]+solutieFinala[0],solutieCurenta[1]+solutieFinala[1]+1,solutieCurenta[2]+solutieFinala[2],solutieCurenta[3]+solutieFinala[3]],nr);
+  assert forall solutieCurenta :: esteSolutieValida(solutieCurenta) && esteSolutie(solutieCurenta, rest - 5) ==> 
+          esteSolutieOptima([solutieCurenta[0] + solutieFinala[0], solutieCurenta[1] + solutieFinala[1] + 1,
+          solutieCurenta[2] + solutieFinala[2], solutieCurenta[3] + solutieFinala[3], solutieCurenta[4] + solutieFinala[4]], suma);
 
 }
 
-lemma aux2(copie:int,solutieCurenta:seq<int>)
-  requires 10 <= copie < 20
+
+
+lemma exchangeArgumentCaz10(rest : int, solutieCurenta : seq<int>)
+  requires 10 <= rest < 20
   requires esteSolutieValida(solutieCurenta)
-  requires esteSolutieOptima(solutieCurenta,copie-10)
-  ensures esteSolutieOptima([solutieCurenta[0], solutieCurenta[1],solutieCurenta[2]+1,solutieCurenta[3]],copie)
+  requires esteSolutieOptima(solutieCurenta, rest - 10)
+  ensures esteSolutieOptima([solutieCurenta[0], solutieCurenta[1], solutieCurenta[2] + 1, solutieCurenta[3], solutieCurenta[4]], rest)
 {
 
-    assert esteSolutie([solutieCurenta[0], solutieCurenta[1],solutieCurenta[2]+1,solutieCurenta[3]],copie);
-    if(!esteSolutieOptima([solutieCurenta[0], solutieCurenta[1],solutieCurenta[2]+1,solutieCurenta[3]],copie))
+    assert esteSolutie([solutieCurenta[0], solutieCurenta[1], solutieCurenta[2] + 1, solutieCurenta[3], solutieCurenta[4]], rest);
+    if(!esteSolutieOptima([solutieCurenta[0], solutieCurenta[1], solutieCurenta[2] + 1, solutieCurenta[3], solutieCurenta[4]], rest))
     {
-      var solopt :|esteSolutieValida(solopt) && esteSolutie(solopt,copie) && cost(solopt)<cost([solutieCurenta[0], solutieCurenta[1],solutieCurenta[2]+1,solutieCurenta[3]]);
-      assert cost([solutieCurenta[0], solutieCurenta[1],solutieCurenta[2]+1,solutieCurenta[3]]) == cost(solutieCurenta)+1;
-      assert solopt[3]==0;
-      if(solopt[2]>=1)
+      var solutieOptima :|esteSolutieValida(solutieOptima) && esteSolutie(solutieOptima, rest) && 
+        cost(solutieOptima) < cost([solutieCurenta[0], solutieCurenta[1], solutieCurenta[2] + 1, solutieCurenta[3], solutieCurenta[4]]);
+      assert cost([solutieCurenta[0], solutieCurenta[1], solutieCurenta[2] + 1, solutieCurenta[3], solutieCurenta[4]]) == cost(solutieCurenta) + 1;
+      assert solutieOptima[3] == 0;
+      assert solutieOptima[4] == 0;
+      if(solutieOptima[2] >= 1)
       {
-        var solopt' := [solopt[0],solopt[1],solopt[2]-1,solopt[3]];
-        assert esteSolutie(solopt',copie-10);
-        assert cost(solopt') == cost(solopt)-1;
-        assert cost(solopt)-1 < cost(solutieCurenta);
+        var solutieOptima' := [solutieOptima[0], solutieOptima[1], solutieOptima[2] - 1, solutieOptima[3], solutieOptima[4]];
+        assert esteSolutie(solutieOptima', rest - 10);
+        assert cost(solutieOptima') == cost(solutieOptima) - 1;
+        assert cost(solutieOptima) - 1 < cost(solutieCurenta);
         assert false;
       }
-      else if(solopt[1]>=2)
+      else if(solutieOptima[1] >= 2)
       {
-        var solopt' := [solopt[0],solopt[1]-2,solopt[2],solopt[3]];
-        assert esteSolutie(solopt',copie-10);
-        assert cost(solopt') == cost(solopt)-2;
-        assert cost(solopt)-2 < cost(solutieCurenta);
+        var solutieOptima' := [solutieOptima[0], solutieOptima[1] - 2, solutieOptima[2], solutieOptima[3], solutieOptima[4]];
+        assert esteSolutie(solutieOptima', rest - 10);
+        assert cost(solutieOptima') == cost(solutieOptima) - 2;
+        assert cost(solutieOptima) - 2 < cost(solutieCurenta);
         assert false;
-      }else if(solopt[1]>=1 && solopt[0]>=5 )
+      }else if(solutieOptima[1] >= 1 && solutieOptima[0] >= 5)
       {
-        var solopt' := [solopt[0]-5,solopt[1]-1,solopt[2],solopt[3]];
-        assert esteSolutie(solopt',copie-10);
-        assert cost(solopt') == cost(solopt)-6;
-        assert cost(solopt)-6 < cost(solutieCurenta);
+        var solutieOptima' := [solutieOptima[0] - 5, solutieOptima[1] - 1, solutieOptima[2], solutieOptima[3], solutieOptima[4]];
+        assert esteSolutie(solutieOptima', rest - 10);
+        assert cost(solutieOptima') == cost(solutieOptima) - 6;
+        assert cost(solutieOptima) - 6 < cost(solutieCurenta);
         assert false;
       }
-      else if(solopt[0]>=10 )
+      else if(solutieOptima[0] >= 10)
       {
-        var solopt' := [solopt[0]-10,solopt[1],solopt[2],solopt[3]];
-        assert esteSolutie(solopt',copie-10);
-        assert cost(solopt') == cost(solopt)-10;
-        assert cost(solopt)-10 < cost(solutieCurenta);
+        var solutieOptima' := [solutieOptima[0] - 10, solutieOptima[1], solutieOptima[2], solutieOptima[3], solutieOptima[4]];
+        assert esteSolutie(solutieOptima', rest - 10);
+        assert cost(solutieOptima') == cost(solutieOptima) - 10;
+        assert cost(solutieOptima) - 10 < cost(solutieCurenta);
         assert false;
       }
       else{
@@ -180,318 +191,793 @@ lemma aux2(copie:int,solutieCurenta:seq<int>)
 
 
 
-lemma cazMaxim10(copie: int, nr: int, solutieFinala: seq<int>)
-  requires 10 <= copie < 20 
+lemma cazMaxim10(rest : int, suma : int, solutieFinala : seq<int>)
+  requires 10 <= rest < 20 
   requires esteSolutieValida(solutieFinala) 
-  requires INV(copie,nr,solutieFinala)
-  ensures INV(copie-10,nr,[solutieFinala[0],solutieFinala[1],solutieFinala[2]+1,solutieFinala[3]])
+  requires INV(rest, suma, solutieFinala)
+  ensures INV(rest - 10, suma, [solutieFinala[0], solutieFinala[1], solutieFinala[2] + 1, solutieFinala[3], solutieFinala[4]])
 {
 
- forall solutieCurenta | esteSolutieValida(solutieCurenta) && esteSolutieOptima(solutieCurenta,copie-10) 
-          ensures esteSolutieOptima([solutieFinala[0]+solutieCurenta[0],solutieFinala[1]+solutieCurenta[1],
-          solutieCurenta[2]+solutieFinala[2]+1,solutieCurenta[3]+solutieFinala[3]],nr)
+ forall solutieCurenta | esteSolutieValida(solutieCurenta) && esteSolutieOptima(solutieCurenta, rest - 10) 
+          ensures esteSolutieOptima([solutieFinala[0] + solutieCurenta[0], solutieFinala[1] + solutieCurenta[1],
+          solutieCurenta[2] + solutieFinala[2] + 1,solutieCurenta[3] + solutieFinala[3], solutieCurenta[4] + solutieFinala[4]], suma)
   {
-    assert esteSolutie(solutieCurenta,copie-10);
-    assert esteSolutie([solutieCurenta[0], solutieCurenta[1],solutieCurenta[2]+1,solutieCurenta[3]],copie);
+    assert esteSolutie(solutieCurenta, rest - 10);
+    assert esteSolutie([solutieCurenta[0], solutieCurenta[1], solutieCurenta[2] + 1,solutieCurenta[3], solutieCurenta[4]], rest);
 
-    aux2(copie,solutieCurenta);
+    exchangeArgumentCaz10(rest, solutieCurenta);
 
-    assert esteSolutieOptima([solutieCurenta[0], solutieCurenta[1],solutieCurenta[2]+1,solutieCurenta[3]],copie);
+    assert esteSolutieOptima([solutieCurenta[0], solutieCurenta[1], solutieCurenta[2] + 1, solutieCurenta[3], solutieCurenta[4]], rest);
 
-    assert forall solutieOarecare :: esteSolutieValida(solutieOarecare)  && esteSolutie(solutieOarecare,copie-10) 
+    assert forall solutieOarecare :: esteSolutieValida(solutieOarecare) && esteSolutie(solutieOarecare, rest - 10) 
           ==> cost(solutieOarecare) >= cost(solutieCurenta);
     
 
-    assert esteSolutie([solutieFinala[0]+solutieCurenta[0],solutieFinala[1]+solutieCurenta[1],1+solutieFinala[2]+solutieCurenta[2],solutieFinala[3]+solutieCurenta[3]],nr);
+    assert esteSolutie([solutieFinala[0] + solutieCurenta[0], solutieFinala[1] + solutieCurenta[1], 1 + solutieFinala[2] + solutieCurenta[2], solutieFinala[3] + solutieCurenta[3],solutieFinala[4] + solutieCurenta[4]], suma);
 
-    assert forall solutieOarecare :: esteSolutieValida(solutieOarecare) && esteSolutie(solutieOarecare,nr)
-          ==> cost(solutieOarecare) >= cost([solutieCurenta[0]+solutieFinala[0],solutieCurenta[1]+solutieFinala[1],
-                                        solutieCurenta[2]+solutieFinala[2]+1,solutieCurenta[3]+solutieFinala[3]]);
+    assert forall solutieOarecare :: esteSolutieValida(solutieOarecare) && esteSolutie(solutieOarecare, suma)
+          ==> cost(solutieOarecare) >= cost([solutieCurenta[0] + solutieFinala[0], solutieCurenta[1] + solutieFinala[1],
+                                        solutieCurenta[2] + solutieFinala[2] + 1,solutieCurenta[3] + solutieFinala[3], solutieCurenta[4] + solutieFinala[4]]);
   }
 
-  assert forall solutieCurenta :: esteSolutieValida(solutieCurenta) && esteSolutieOptima(solutieCurenta,copie-10) ==> 
-          esteSolutieOptima([solutieCurenta[0]+solutieFinala[0],solutieCurenta[1]+solutieFinala[1],
-                            solutieCurenta[2]+solutieFinala[2]+1,solutieCurenta[3]+solutieFinala[3]],nr);
+  assert forall solutieCurenta :: esteSolutieValida(solutieCurenta) && esteSolutieOptima(solutieCurenta, rest - 10) ==> 
+          esteSolutieOptima([solutieCurenta[0] + solutieFinala[0], solutieCurenta[1] + solutieFinala[1],
+                            solutieCurenta[2] + solutieFinala[2] + 1, solutieCurenta[3] + solutieFinala[3], solutieCurenta[4] + solutieFinala[4]], suma);
 
 }
 
 
 
-lemma B(copie:int,nr: int,solutieOarecare : seq<int>, solutieCurenta: seq<int>)
+lemma exchangeArgumentCaz20(rest : int, solutieCurenta : seq<int>)
+  requires 20 <= rest < 50
+  requires esteSolutieValida(solutieCurenta)
+  requires esteSolutieOptima(solutieCurenta, rest - 20)
+  ensures esteSolutieOptima([solutieCurenta[0], solutieCurenta[1], solutieCurenta[2], 1 + solutieCurenta[3], solutieCurenta[4]], rest)
+{
+
+    assert esteSolutie([solutieCurenta[0], solutieCurenta[1], solutieCurenta[2], 1 + solutieCurenta[3], solutieCurenta[4]], rest);
+    if(!esteSolutieOptima([solutieCurenta[0], solutieCurenta[1], solutieCurenta[2], 1 + solutieCurenta[3], solutieCurenta[4]], rest))
+    {
+      var solutieOptima :|esteSolutieValida(solutieOptima) && esteSolutie(solutieOptima, rest) && cost(solutieOptima) < cost([solutieCurenta[0], solutieCurenta[1], solutieCurenta[2], 1 + solutieCurenta[3], solutieCurenta[4]]);
+      assert cost([solutieCurenta[0], solutieCurenta[1], solutieCurenta[2], 1 + solutieCurenta[3], solutieCurenta[4]]) == cost(solutieCurenta) + 1;
+      assert solutieOptima[4] == 0;
+      if(solutieOptima[3] >= 1)
+      {
+        var solutieOptima' := [solutieOptima[0], solutieOptima[1], solutieOptima[2], solutieOptima[3] - 1, solutieOptima[4]];
+        assert esteSolutie(solutieOptima', rest - 20);
+        assert cost(solutieOptima') == cost(solutieOptima) - 1;
+        assert cost(solutieOptima) - 1 < cost(solutieCurenta);
+        assert false;
+      }
+      else if(solutieOptima[2] >= 2)
+      {
+        var solutieOptima' := [solutieOptima[0], solutieOptima[1], solutieOptima[2] - 2, solutieOptima[3], solutieOptima[4]];
+        assert esteSolutie(solutieOptima', rest - 20);
+        assert cost(solutieOptima') == cost(solutieOptima) - 2;
+        assert cost(solutieOptima) - 2 < cost(solutieCurenta);
+        assert false;
+      }
+      else if(solutieOptima[2] >= 1 && solutieOptima[1] >= 2)
+      {       
+        var solutieOptima' := [solutieOptima[0], solutieOptima[1] - 2, solutieOptima[2] - 1, solutieOptima[3], solutieOptima[4]];
+        assert esteSolutie(solutieOptima', rest - 20);
+        assert cost(solutieOptima') == cost(solutieOptima) - 3;
+        assert cost(solutieOptima) - 3 < cost(solutieCurenta);
+        assert false;
+      }
+      else if(solutieOptima[2] >= 1 && solutieOptima[1] >= 1 && solutieOptima[0] >= 5)
+      {
+        var solutieOptima' := [solutieOptima[0] - 5, solutieOptima[1] - 1, solutieOptima[2] - 1, solutieOptima[3], solutieOptima[4]];
+        assert esteSolutie(solutieOptima', rest - 20);
+        assert cost(solutieOptima') == cost(solutieOptima) - 7;
+        assert cost(solutieOptima) - 7 < cost(solutieCurenta);
+        assert false;
+      }
+      else if(solutieOptima[1] >= 4)
+      {
+        var solutieOptima' := [solutieOptima[0], solutieOptima[1] - 4, solutieOptima[2], solutieOptima[3], solutieOptima[4]];
+        assert esteSolutie(solutieOptima', rest - 20);
+        assert cost(solutieOptima') == cost(solutieOptima) - 4;
+        assert cost(solutieOptima) - 4 < cost(solutieCurenta);
+        assert false;
+      }
+      else if(solutieOptima[1] >= 3 && solutieOptima[0] >= 5)
+      {
+        var solutieOptima' := [solutieOptima[0] - 5, solutieOptima[1] - 3, solutieOptima[2], solutieOptima[3], solutieOptima[4]];
+        assert esteSolutie(solutieOptima', rest - 20);
+        assert cost(solutieOptima') == cost(solutieOptima) - 8;
+        assert cost(solutieOptima) - 8 < cost(solutieCurenta);
+        assert false;
+      }
+      else if(solutieOptima[1] >= 2 && solutieOptima[0] >= 10)
+      {
+        var solutieOptima' := [solutieOptima[0] - 10, solutieOptima[1] - 2, solutieOptima[2], solutieOptima[3], solutieOptima[4]];
+        assert esteSolutie(solutieOptima', rest - 20);
+        assert cost(solutieOptima') == cost(solutieOptima) - 12;
+        assert cost(solutieOptima) - 12 < cost(solutieCurenta);
+        assert false;
+      }
+      else if(solutieOptima[1] >= 1 && solutieOptima[0] >= 15)
+      {
+        var solutieOptima' := [solutieOptima[0] - 15, solutieOptima[1] - 1, solutieOptima[2], solutieOptima[3], solutieOptima[4]];
+        assert esteSolutie(solutieOptima', rest - 20);
+        assert cost(solutieOptima') == cost(solutieOptima) - 16;
+        assert cost(solutieOptima) - 16 < cost(solutieCurenta);
+        assert false;
+      }
+      else if(solutieOptima[0] >= 20)
+      {
+        var solutieOptima' := [solutieOptima[0] - 20, solutieOptima[1], solutieOptima[2], solutieOptima[3], solutieOptima[4]];
+        assert esteSolutie(solutieOptima', rest - 20);
+        assert cost(solutieOptima') == cost(solutieOptima) - 20;
+        assert cost(solutieOptima) - 20 < cost(solutieCurenta);
+        assert false;
+      }
+      else if(solutieOptima[2] >= 1 && solutieOptima[0] >= 10)
+      {
+        var solutieOptima' := [solutieOptima[0] - 10, solutieOptima[1], solutieOptima[2] - 1, solutieOptima[3], solutieOptima[4]];
+        assert esteSolutie(solutieOptima', rest - 20);
+        assert cost(solutieOptima') == cost(solutieOptima) - 11;
+        assert cost(solutieOptima) - 11 < cost(solutieCurenta);
+        assert false;
+      }
+      else{
+        assert false;
+      }
+    }
+}
+
+
+
+lemma cazMaxim20(rest : int, suma : int, solutieFinala : seq<int>)
+  requires 20 <= rest < 50 
+  requires esteSolutieValida(solutieFinala) 
+  requires INV(rest, suma, solutieFinala)
+  ensures INV(rest - 20, suma, [solutieFinala[0], solutieFinala[1], solutieFinala[2], solutieFinala[3] + 1, solutieFinala[4]])
+{
+
+ forall solutieCurenta | esteSolutieValida(solutieCurenta) && esteSolutieOptima(solutieCurenta, rest - 20) 
+          ensures esteSolutieOptima([solutieFinala[0] + solutieCurenta[0], solutieFinala[1] + solutieCurenta[1],
+          solutieCurenta[2] + solutieFinala[2], solutieCurenta[3] + solutieFinala[3] + 1, solutieCurenta[4] + solutieFinala[4]], suma)
+  {
+    assert esteSolutie(solutieCurenta, rest - 20);
+    assert esteSolutie([solutieCurenta[0], solutieCurenta[1], solutieCurenta[2], solutieCurenta[3] + 1, solutieCurenta[4]], rest);
+
+    exchangeArgumentCaz20(rest, solutieCurenta);
+
+    assert esteSolutieOptima([solutieCurenta[0], solutieCurenta[1], solutieCurenta[2], 1 + solutieCurenta[3], solutieCurenta[4]], rest);
+
+    assert forall solutieOarecare :: esteSolutieValida(solutieOarecare) && esteSolutie(solutieOarecare, rest - 20) 
+          ==> cost(solutieOarecare) >= cost(solutieCurenta);
+    
+
+    assert esteSolutie([solutieFinala[0] + solutieCurenta[0], solutieFinala[1] + solutieCurenta[1], solutieFinala[2] + solutieCurenta[2], 1 + solutieFinala[3] + solutieCurenta[3], solutieFinala[4] + solutieCurenta[4]], suma);
+
+    assert forall solutieOarecare :: esteSolutieValida(solutieOarecare) && esteSolutie(solutieOarecare, suma)
+          ==> cost(solutieOarecare) >= cost([solutieCurenta[0] + solutieFinala[0], solutieCurenta[1] + solutieFinala[1],
+                                        solutieCurenta[2] + solutieFinala[2], 1 + solutieCurenta[3] + solutieFinala[3], solutieCurenta[4] + solutieFinala[4]]);
+  }
+
+  assert forall solutieCurenta :: esteSolutieValida(solutieCurenta) && esteSolutieOptima(solutieCurenta, rest - 20) ==> 
+          esteSolutieOptima([solutieCurenta[0] + solutieFinala[0], solutieCurenta[1] + solutieFinala[1],
+                            solutieCurenta[2] + solutieFinala[2], 1 + solutieCurenta[3] + solutieFinala[3], solutieCurenta[4] + solutieFinala[4]], suma);
+
+}
+
+
+
+
+lemma exchangeArgumentCaz50(rest : int, suma : int, solutieOarecare : seq<int>, solutieCurenta : seq<int>)
   requires esteSolutieValida(solutieOarecare)
   requires esteSolutieValida(solutieCurenta)
-  requires copie >= 20
-  requires esteSolutie(solutieOarecare,copie)
-  requires esteSolutie(solutieCurenta,copie-20)
-  requires esteSolutieOptima(solutieCurenta,copie-20)
-  ensures cost(solutieOarecare) >= cost([solutieCurenta[0],solutieCurenta[1],solutieCurenta[2],1+solutieCurenta[3]])
-  decreases solutieOarecare[0],solutieOarecare[1],solutieOarecare[2]
+  requires rest >= 50
+  requires esteSolutie(solutieOarecare, rest)
+  requires esteSolutie(solutieCurenta, rest - 50)
+  requires esteSolutieOptima(solutieCurenta, rest - 50)
+  ensures cost(solutieOarecare) >= cost([solutieCurenta[0], solutieCurenta[1], solutieCurenta[2], solutieCurenta[3], 1 + solutieCurenta[4]])
+  decreases solutieOarecare[0] + solutieOarecare[1] + solutieOarecare[2] + solutieOarecare[3]
 {
-  assert esteSolutie(solutieOarecare,copie);
-  assert esteSolutie([solutieCurenta[0],solutieCurenta[1],solutieCurenta[2],solutieCurenta[3]+1],copie);
+  assert esteSolutie(solutieOarecare, rest);
+  assert esteSolutie([solutieCurenta[0], solutieCurenta[1], solutieCurenta[2], solutieCurenta[3], 1 + solutieCurenta[4]], rest);
 
-  if(cost(solutieOarecare) < cost([solutieCurenta[0],solutieCurenta[1],solutieCurenta[2],1+solutieCurenta[3]]))
+  if(cost(solutieOarecare) < cost([solutieCurenta[0], solutieCurenta[1], solutieCurenta[2], solutieCurenta[3], 1 + solutieCurenta[4]]))
   {
-    if(solutieOarecare[3] > (solutieCurenta[3]+1))
+    if(solutieOarecare[4] > solutieCurenta[4] + 1)
     {
-      assert cost([solutieOarecare[0],solutieOarecare[1],solutieOarecare[2],solutieOarecare[3]-1]) < cost(solutieCurenta);
-      assert esteSolutieOptima([solutieOarecare[0],solutieOarecare[1],solutieOarecare[2],solutieOarecare[3]-1],(copie-20));
+      assert cost([solutieOarecare[0], solutieOarecare[1], solutieOarecare[2], solutieOarecare[3], solutieOarecare[4] - 1]) < cost(solutieCurenta);
+      assert esteSolutieOptima([solutieOarecare[0], solutieOarecare[1], solutieOarecare[2], solutieOarecare[3], solutieOarecare[4] - 1], rest - 50);
+      assert false;
+    }
+    else if(solutieOarecare[4] < solutieCurenta[4] + 1)
+    {
+      assert (solutieOarecare[0] + (5 * solutieOarecare[1])+(10 * solutieOarecare[2]) + (20 * solutieOarecare[3])) >= 50;
+
+      if(solutieOarecare[2] >= 1 && solutieOarecare[3] >= 2)
+      {
+          var nouaSolutieOarecare := [solutieOarecare[0], solutieOarecare[1], solutieOarecare[2] - 1, solutieOarecare[3] - 2, solutieOarecare[4] + 1];
+          exchangeArgumentCaz50(rest, suma, nouaSolutieOarecare, solutieCurenta);
+      }
+      else if(solutieOarecare[2] >= 3 && solutieOarecare[3] >= 1)
+      {
+          var nouaSolutieOarecare := [solutieOarecare[0], solutieOarecare[1], solutieOarecare[2] - 3, solutieOarecare[3] - 1, solutieOarecare[4] + 1];
+          exchangeArgumentCaz50(rest, suma, nouaSolutieOarecare, solutieCurenta);
+      }
+      else if(solutieOarecare[2] >= 5)
+      {
+          var nouaSolutieOarecare := [solutieOarecare[0], solutieOarecare[1], solutieOarecare[2] - 5, solutieOarecare[3], solutieOarecare[4] + 1];
+          exchangeArgumentCaz50(rest, suma, nouaSolutieOarecare, solutieCurenta);
+      }
+      else if(solutieOarecare[1] >= 10)
+      {
+          var nouaSolutieOarecare := [solutieOarecare[0], solutieOarecare[1] - 10, solutieOarecare[2], solutieOarecare[3], solutieOarecare[4] + 1];
+          exchangeArgumentCaz50(rest, suma, nouaSolutieOarecare, solutieCurenta);
+      }
+      else if(solutieOarecare[1] >= 8 && solutieOarecare[2] >= 1)
+      {
+          var nouaSolutieOarecare := [solutieOarecare[0], solutieOarecare[1] - 8, solutieOarecare[2] - 1, solutieOarecare[3], solutieOarecare[4] + 1];
+          exchangeArgumentCaz50(rest, suma, nouaSolutieOarecare, solutieCurenta);
+      }
+      else if(solutieOarecare[1] >= 6 && solutieOarecare[2] >= 2)
+      {
+          var nouaSolutieOarecare := [solutieOarecare[0], solutieOarecare[1] - 6, solutieOarecare[2] - 2, solutieOarecare[3], solutieOarecare[4] + 1];
+          exchangeArgumentCaz50(rest, suma, nouaSolutieOarecare, solutieCurenta);
+      }
+      else if(solutieOarecare[1] >= 6 && solutieOarecare[3] >= 1)
+      {
+          var nouaSolutieOarecare := [solutieOarecare[0], solutieOarecare[1] - 6, solutieOarecare[2], solutieOarecare[3] - 1, solutieOarecare[4] + 1];
+          exchangeArgumentCaz50(rest, suma, nouaSolutieOarecare, solutieCurenta);
+      }
+      else if(solutieOarecare[1] >= 4 && solutieOarecare[2] >= 3)
+      {
+          var nouaSolutieOarecare := [solutieOarecare[0], solutieOarecare[1] - 4, solutieOarecare[2] - 3, solutieOarecare[3], solutieOarecare[4] + 1];
+          exchangeArgumentCaz50(rest, suma, nouaSolutieOarecare, solutieCurenta);
+      }
+      else if(solutieOarecare[1] >= 4 && solutieOarecare[2] >= 1 && solutieOarecare[3] >=1)
+      {
+          var nouaSolutieOarecare := [solutieOarecare[0], solutieOarecare[1] - 4, solutieOarecare[2] - 1, solutieOarecare[3] - 1, solutieOarecare[4] + 1];
+          exchangeArgumentCaz50(rest, suma, nouaSolutieOarecare, solutieCurenta);
+      }
+      else if(solutieOarecare[1] >= 2 && solutieOarecare[2] >= 4)
+      {
+          var nouaSolutieOarecare := [solutieOarecare[0], solutieOarecare[1] - 2, solutieOarecare[2] - 4, solutieOarecare[3], solutieOarecare[4] + 1];
+          exchangeArgumentCaz50(rest, suma, nouaSolutieOarecare, solutieCurenta);
+      }
+      else if(solutieOarecare[1] >= 2 && solutieOarecare[2] >= 2 && solutieOarecare[3] >= 1)
+      {
+          var nouaSolutieOarecare := [solutieOarecare[0], solutieOarecare[1] - 2, solutieOarecare[2] - 2, solutieOarecare[3] - 1, solutieOarecare[4] + 1];
+          exchangeArgumentCaz50(rest, suma, nouaSolutieOarecare, solutieCurenta);
+      }
+      else if(solutieOarecare[1] >= 2 && solutieOarecare[3] >= 2)
+      {
+          var nouaSolutieOarecare := [solutieOarecare[0],solutieOarecare[1] - 2, solutieOarecare[2], solutieOarecare[3] - 2,solutieOarecare[4] + 1];
+          exchangeArgumentCaz50(rest, suma, nouaSolutieOarecare, solutieCurenta);
+      }
+      else if(solutieOarecare[0] >= 50)
+      {
+          var nouaSolutieOarecare := [solutieOarecare[0] - 50, solutieOarecare[1], solutieOarecare[2], solutieOarecare[3], solutieOarecare[4] + 1];
+          exchangeArgumentCaz50(rest, suma, nouaSolutieOarecare, solutieCurenta);
+      }
+      else if(solutieOarecare[0] >= 45 && solutieOarecare[1] >= 1)
+      {
+          var nouaSolutieOarecare := [solutieOarecare[0] - 45, solutieOarecare[1] - 1, solutieOarecare[2], solutieOarecare[3], solutieOarecare[4] + 1];
+          exchangeArgumentCaz50(rest, suma, nouaSolutieOarecare, solutieCurenta);
+      }
+      else if(solutieOarecare[0] >= 40 && solutieOarecare[1] >= 2)
+      {
+          var nouaSolutieOarecare := [solutieOarecare[0] - 40, solutieOarecare[1] - 2, solutieOarecare[2], solutieOarecare[3], solutieOarecare[4] + 1];
+          exchangeArgumentCaz50(rest, suma, nouaSolutieOarecare, solutieCurenta);
+      }
+      else if(solutieOarecare[0] >= 40 && solutieOarecare[2] >= 1)
+      {
+          var nouaSolutieOarecare := [solutieOarecare[0] - 40, solutieOarecare[1], solutieOarecare[2] - 1, solutieOarecare[3], solutieOarecare[4] + 1];
+          exchangeArgumentCaz50(rest, suma, nouaSolutieOarecare, solutieCurenta);
+      }
+      else if(solutieOarecare[0] >= 35 && solutieOarecare[1] >= 3)
+      {
+          var nouaSolutieOarecare := [solutieOarecare[0] - 35, solutieOarecare[1] - 3, solutieOarecare[2], solutieOarecare[3], solutieOarecare[4] + 1];
+          exchangeArgumentCaz50(rest, suma, nouaSolutieOarecare, solutieCurenta);
+      }
+      else if(solutieOarecare[0] >= 35 && solutieOarecare[1] >= 1 && solutieOarecare[2] >= 1)
+      {
+          var nouaSolutieOarecare := [solutieOarecare[0] - 35, solutieOarecare[1] - 1, solutieOarecare[2] - 1, solutieOarecare[3], solutieOarecare[4] + 1];
+          exchangeArgumentCaz50(rest, suma, nouaSolutieOarecare, solutieCurenta);
+      }
+      else if(solutieOarecare[0] >= 30 && solutieOarecare[1] >= 4)
+      {
+          var nouaSolutieOarecare := [solutieOarecare[0] - 30, solutieOarecare[1] - 4, solutieOarecare[2], solutieOarecare[3], solutieOarecare[4] + 1];
+          exchangeArgumentCaz50(rest, suma, nouaSolutieOarecare, solutieCurenta);
+      }
+      else if(solutieOarecare[0] >= 30 && solutieOarecare[1] >= 2 && solutieOarecare[2] >= 1)
+      {
+          var nouaSolutieOarecare := [solutieOarecare[0] - 30, solutieOarecare[1] - 2, solutieOarecare[2] - 1, solutieOarecare[3], solutieOarecare[4] + 1];
+          exchangeArgumentCaz50(rest, suma, nouaSolutieOarecare, solutieCurenta);
+      }
+      else if(solutieOarecare[0] >= 30 && solutieOarecare[2] >= 2)
+      {
+          var nouaSolutieOarecare := [solutieOarecare[0] - 30, solutieOarecare[1], solutieOarecare[2] - 2, solutieOarecare[3], solutieOarecare[4] + 1];
+          exchangeArgumentCaz50(rest, suma, nouaSolutieOarecare, solutieCurenta);
+      }
+      else if(solutieOarecare[0] >= 30 && solutieOarecare[3] >= 1)
+      {
+          var nouaSolutieOarecare := [solutieOarecare[0] - 30, solutieOarecare[1], solutieOarecare[2], solutieOarecare[3] - 1, solutieOarecare[4] + 1];
+          exchangeArgumentCaz50(rest, suma, nouaSolutieOarecare, solutieCurenta);
+      }
+      else if(solutieOarecare[0] >= 25 && solutieOarecare[1] >= 5)
+      {
+          var nouaSolutieOarecare := [solutieOarecare[0] - 25, solutieOarecare[1] - 5, solutieOarecare[2], solutieOarecare[3], solutieOarecare[4] + 1];
+          exchangeArgumentCaz50(rest, suma, nouaSolutieOarecare, solutieCurenta);
+      }
+      else if(solutieOarecare[0] >= 25 && solutieOarecare[1] >= 3 &&solutieOarecare[2] >= 1)
+      {
+          var nouaSolutieOarecare := [solutieOarecare[0] - 25, solutieOarecare[1] - 3, solutieOarecare[2] - 1, solutieOarecare[3], solutieOarecare[4] + 1];
+          exchangeArgumentCaz50(rest, suma, nouaSolutieOarecare, solutieCurenta);
+      }
+      else if(solutieOarecare[0] >= 25 && solutieOarecare[1] >= 1 &&solutieOarecare[2] >= 2)
+      {
+          var nouaSolutieOarecare := [solutieOarecare[0] - 25, solutieOarecare[1] - 1, solutieOarecare[2] - 2, solutieOarecare[3], solutieOarecare[4] + 1];
+          exchangeArgumentCaz50(rest, suma, nouaSolutieOarecare, solutieCurenta);
+      }
+      else if(solutieOarecare[0] >= 25 && solutieOarecare[1] >= 1 && solutieOarecare[3] >= 1)
+      {
+          var nouaSolutieOarecare := [solutieOarecare[0] - 25, solutieOarecare[1] - 1, solutieOarecare[2], solutieOarecare[3] - 1, solutieOarecare[4] + 1];
+          exchangeArgumentCaz50(rest, suma, nouaSolutieOarecare, solutieCurenta);
+      }
+      else if(solutieOarecare[0] >= 20 && solutieOarecare[1] >= 6)
+      {
+          var nouaSolutieOarecare := [solutieOarecare[0] - 20, solutieOarecare[1] - 6, solutieOarecare[2], solutieOarecare[3], solutieOarecare[4] + 1];
+          exchangeArgumentCaz50(rest, suma, nouaSolutieOarecare, solutieCurenta);
+      }
+      else if(solutieOarecare[0] >= 20 && solutieOarecare[1] >= 4 && solutieOarecare[2] >= 1)
+      {
+          var nouaSolutieOarecare := [solutieOarecare[0] - 20, solutieOarecare[1] - 4, solutieOarecare[2] - 1, solutieOarecare[3], solutieOarecare[4] + 1];
+          exchangeArgumentCaz50(rest, suma, nouaSolutieOarecare, solutieCurenta);
+      }
+      else if(solutieOarecare[0] >= 20 && solutieOarecare[1] >= 2 && solutieOarecare[2] >= 2)
+      {
+          var nouaSolutieOarecare := [solutieOarecare[0] - 20, solutieOarecare[1] - 2, solutieOarecare[2] - 2, solutieOarecare[3], solutieOarecare[4] + 1];
+          exchangeArgumentCaz50(rest, suma, nouaSolutieOarecare, solutieCurenta);
+      }
+      else if(solutieOarecare[0] >= 20 && solutieOarecare[1] >= 2 && solutieOarecare[3] >= 1)
+      {
+          var nouaSolutieOarecare := [solutieOarecare[0] - 20, solutieOarecare[1] - 2, solutieOarecare[2], solutieOarecare[3] - 1, solutieOarecare[4] + 1];
+          exchangeArgumentCaz50(rest, suma, nouaSolutieOarecare, solutieCurenta);
+      }
+      else if(solutieOarecare[0] >= 20 && solutieOarecare[2] >= 3)
+      {
+          var nouaSolutieOarecare := [solutieOarecare[0] - 20, solutieOarecare[1], solutieOarecare[2] - 3, solutieOarecare[3], solutieOarecare[4] + 1];
+          exchangeArgumentCaz50(rest, suma, nouaSolutieOarecare, solutieCurenta);
+      }
+      else if(solutieOarecare[0] >= 20 && solutieOarecare[2] >= 1 && solutieOarecare[3] >= 1)
+      {
+          var nouaSolutieOarecare := [solutieOarecare[0] - 20, solutieOarecare[1], solutieOarecare[2] - 1, solutieOarecare[3] - 1, solutieOarecare[4] + 1];
+          exchangeArgumentCaz50(rest, suma, nouaSolutieOarecare, solutieCurenta);
+      }
+      else if(solutieOarecare[0] >= 15 && solutieOarecare[1] >= 7)
+      {
+          var nouaSolutieOarecare := [solutieOarecare[0] - 15, solutieOarecare[1] - 7, solutieOarecare[2], solutieOarecare[3], solutieOarecare[4] + 1];
+          exchangeArgumentCaz50(rest, suma, nouaSolutieOarecare, solutieCurenta);
+      }
+      else if(solutieOarecare[0] >= 15 && solutieOarecare[1] >= 5 && solutieOarecare[2] >= 1)
+      {
+          var nouaSolutieOarecare := [solutieOarecare[0] - 15, solutieOarecare[1] - 5, solutieOarecare[2] - 1, solutieOarecare[3], solutieOarecare[4] + 1];
+          exchangeArgumentCaz50(rest, suma, nouaSolutieOarecare, solutieCurenta);
+      }
+      else if(solutieOarecare[0] >= 15 && solutieOarecare[1] >= 3 && solutieOarecare[2] >= 2)
+      {
+          var nouaSolutieOarecare := [solutieOarecare[0] - 15, solutieOarecare[1] - 3, solutieOarecare[2] - 2, solutieOarecare[3], solutieOarecare[4] + 1];
+          exchangeArgumentCaz50(rest, suma, nouaSolutieOarecare, solutieCurenta);
+      }
+      else if(solutieOarecare[0] >= 15 && solutieOarecare[1] >= 3 && solutieOarecare[3] >= 1)
+      {
+          var nouaSolutieOarecare := [solutieOarecare[0] - 15, solutieOarecare[1] - 3, solutieOarecare[2], solutieOarecare[3] - 1, solutieOarecare[4] + 1];
+          exchangeArgumentCaz50(rest, suma, nouaSolutieOarecare, solutieCurenta);
+      }
+      else if(solutieOarecare[0] >= 15 && solutieOarecare[1] >= 1 && solutieOarecare[2] >= 3)
+      {
+          var nouaSolutieOarecare := [solutieOarecare[0] - 15, solutieOarecare[1] - 1, solutieOarecare[2] - 3, solutieOarecare[3], solutieOarecare[4] + 1];
+          exchangeArgumentCaz50(rest, suma, nouaSolutieOarecare, solutieCurenta);
+      }
+      else if(solutieOarecare[0] >= 15 && solutieOarecare[1] >= 1 && solutieOarecare[2] >= 1 && solutieOarecare[3] >= 1)
+      {
+          var nouaSolutieOarecare := [solutieOarecare[0] - 15, solutieOarecare[1] - 1, solutieOarecare[2] - 1, solutieOarecare[3] - 1, solutieOarecare[4] + 1];
+          exchangeArgumentCaz50(rest, suma, nouaSolutieOarecare, solutieCurenta);
+      }
+      else if(solutieOarecare[0] >= 10 && solutieOarecare[1] >= 8)
+      {
+          var nouaSolutieOarecare := [solutieOarecare[0] - 10, solutieOarecare[1] - 8, solutieOarecare[2], solutieOarecare[3], solutieOarecare[4] + 1];
+          exchangeArgumentCaz50(rest, suma, nouaSolutieOarecare, solutieCurenta);
+      }
+      else if(solutieOarecare[0] >= 10 && solutieOarecare[1] >= 6 && solutieOarecare[2] >= 1)
+      {
+          var nouaSolutieOarecare := [solutieOarecare[0] - 10, solutieOarecare[1] - 6, solutieOarecare[2] - 1, solutieOarecare[3], solutieOarecare[4] + 1];
+          exchangeArgumentCaz50(rest, suma, nouaSolutieOarecare, solutieCurenta);
+      }
+      else if(solutieOarecare[0] >= 10 && solutieOarecare[1] >= 4 && solutieOarecare[2] >= 2)
+      {
+          var nouaSolutieOarecare := [solutieOarecare[0] - 10, solutieOarecare[1] - 4, solutieOarecare[2] - 2, solutieOarecare[3], solutieOarecare[4] + 1];
+          exchangeArgumentCaz50(rest, suma, nouaSolutieOarecare, solutieCurenta);
+      }
+      else if(solutieOarecare[0] >= 10 && solutieOarecare[1] >= 4 && solutieOarecare[3] >= 1)
+      {
+          var nouaSolutieOarecare := [solutieOarecare[0] - 10, solutieOarecare[1] - 4, solutieOarecare[2], solutieOarecare[3] - 1, solutieOarecare[4] + 1];
+          exchangeArgumentCaz50(rest, suma, nouaSolutieOarecare, solutieCurenta);
+      }
+      else if(solutieOarecare[0] >= 10 && solutieOarecare[1] >= 2 && solutieOarecare[2] >= 3)
+      {
+          var nouaSolutieOarecare := [solutieOarecare[0] - 10, solutieOarecare[1] - 2, solutieOarecare[2] - 3, solutieOarecare[3], solutieOarecare[4] + 1];
+          exchangeArgumentCaz50(rest, suma, nouaSolutieOarecare, solutieCurenta);
+      }
+      else if(solutieOarecare[0] >= 10 && solutieOarecare[1] >= 2 && solutieOarecare[2] >= 1 && solutieOarecare[3] >= 1)
+      {
+          var nouaSolutieOarecare := [solutieOarecare[0] - 10, solutieOarecare[1] - 2, solutieOarecare[2] - 1, solutieOarecare[3] - 1, solutieOarecare[4] + 1];
+          exchangeArgumentCaz50(rest, suma, nouaSolutieOarecare, solutieCurenta);
+      }
+      else if(solutieOarecare[0] >= 10 && solutieOarecare[2] >= 4)
+      {
+          var nouaSolutieOarecare := [solutieOarecare[0] - 10, solutieOarecare[1], solutieOarecare[2] - 4, solutieOarecare[3], solutieOarecare[4] + 1];
+          exchangeArgumentCaz50(rest, suma, nouaSolutieOarecare, solutieCurenta);
+      }
+      else if(solutieOarecare[0] >= 10 && solutieOarecare[2] >= 2 && solutieOarecare[3] >= 1)
+      {
+          var nouaSolutieOarecare := [solutieOarecare[0] - 10, solutieOarecare[1], solutieOarecare[2] - 2, solutieOarecare[3] - 1, solutieOarecare[4] + 1];
+          exchangeArgumentCaz50(rest, suma, nouaSolutieOarecare, solutieCurenta);
+      }
+      else if(solutieOarecare[0] >= 10 && solutieOarecare[3] >= 2)
+      {
+          var nouaSolutieOarecare := [solutieOarecare[0] - 10, solutieOarecare[1], solutieOarecare[2], solutieOarecare[3] - 2, solutieOarecare[4] + 1];
+          exchangeArgumentCaz50(rest, suma, nouaSolutieOarecare, solutieCurenta);
+      }
+      else if(solutieOarecare[0] >= 5 && solutieOarecare[1] >= 9)
+      {
+          var nouaSolutieOarecare := [solutieOarecare[0] - 5, solutieOarecare[1] - 9, solutieOarecare[2], solutieOarecare[3], solutieOarecare[4] + 1];
+          exchangeArgumentCaz50(rest, suma, nouaSolutieOarecare, solutieCurenta);
+      }
+      else if(solutieOarecare[0] >= 5 && solutieOarecare[1] >= 7 && solutieOarecare[2] >= 1)
+      {
+          var nouaSolutieOarecare := [solutieOarecare[0] - 5, solutieOarecare[1] - 7, solutieOarecare[2] - 1, solutieOarecare[3], solutieOarecare[4] + 1];
+          exchangeArgumentCaz50(rest, suma, nouaSolutieOarecare, solutieCurenta);
+      }
+      else if(solutieOarecare[0] >= 5 && solutieOarecare[1] >= 5 && solutieOarecare[2] >= 2)
+      {
+          var nouaSolutieOarecare := [solutieOarecare[0] - 5, solutieOarecare[1] - 5, solutieOarecare[2] - 2, solutieOarecare[3], solutieOarecare[4] + 1];
+          exchangeArgumentCaz50(rest, suma, nouaSolutieOarecare, solutieCurenta);
+      }
+      else if(solutieOarecare[0] >= 5 && solutieOarecare[1] >= 5 && solutieOarecare[3] >= 1)
+      {
+          var nouaSolutieOarecare := [solutieOarecare[0] - 5, solutieOarecare[1] - 5, solutieOarecare[2], solutieOarecare[3] - 1, solutieOarecare[4] + 1];
+          exchangeArgumentCaz50(rest, suma, nouaSolutieOarecare, solutieCurenta);
+      }
+      else if(solutieOarecare[0] >= 5 && solutieOarecare[1] >= 3 && solutieOarecare[2] >= 3)
+      {
+          var nouaSolutieOarecare := [solutieOarecare[0] - 5, solutieOarecare[1] - 3, solutieOarecare[2] - 3, solutieOarecare[3], solutieOarecare[4] + 1];
+          exchangeArgumentCaz50(rest, suma, nouaSolutieOarecare, solutieCurenta);
+      }
+      else if(solutieOarecare[0] >= 5 && solutieOarecare[1] >= 3 && solutieOarecare[2] >= 1 && solutieOarecare[3] >= 1)
+      {
+          var nouaSolutieOarecare := [solutieOarecare[0] - 5, solutieOarecare[1] - 3, solutieOarecare[2] - 1, solutieOarecare[3] - 1, solutieOarecare[4] + 1];
+          exchangeArgumentCaz50(rest, suma, nouaSolutieOarecare, solutieCurenta);
+      }
+      else if(solutieOarecare[0] >= 5 && solutieOarecare[1] >= 1 && solutieOarecare[2] >= 4)
+      {
+          var nouaSolutieOarecare := [solutieOarecare[0] - 5, solutieOarecare[1] - 1, solutieOarecare[2] - 4, solutieOarecare[3], solutieOarecare[4] + 1];
+          exchangeArgumentCaz50(rest, suma, nouaSolutieOarecare, solutieCurenta);
+      }
+      else if(solutieOarecare[0] >= 5 && solutieOarecare[1] >= 1 && solutieOarecare[2] >= 2 && solutieOarecare[3] >= 1)
+      {
+          var nouaSolutieOarecare := [solutieOarecare[0] - 5, solutieOarecare[1] - 1, solutieOarecare[2] - 2, solutieOarecare[3] - 1, solutieOarecare[4] + 1];
+          exchangeArgumentCaz50(rest, suma, nouaSolutieOarecare, solutieCurenta);
+      }
+      else if(solutieOarecare[0] >= 5 && solutieOarecare[1] >= 1 && solutieOarecare[3] >= 2)
+      {
+          var nouaSolutieOarecare := [solutieOarecare[0] - 5, solutieOarecare[1] - 1, solutieOarecare[2], solutieOarecare[3] - 2, solutieOarecare[4] + 1];
+          exchangeArgumentCaz50(rest, suma, nouaSolutieOarecare, solutieCurenta);
+      }
+      else{
+          
+          assert solutieOarecare[0] >= 0;
+          assert solutieOarecare[1] >= 0;
+          assert solutieOarecare[2] >= 0;
+          assert solutieOarecare[3] >= 3;
+          if(solutieOarecare[3] >= 3)
+          {
+            var nouaSolutieOarecare := [solutieOarecare[0], solutieOarecare[1], solutieOarecare[2] + 1, solutieOarecare[3] - 3, solutieOarecare[4] + 1];
+            assert cost(nouaSolutieOarecare) < cost(solutieOarecare);
+            exchangeArgumentCaz50(rest, suma, nouaSolutieOarecare, solutieCurenta);
+          }
+      }
+    }
+
+    assert solutieOarecare[4] == (solutieCurenta[4] + 1);
+
+
+    if(solutieOarecare[3] > solutieCurenta[3])
+    {
+      assert cost([solutieOarecare[0], solutieOarecare[1], solutieOarecare[2], solutieOarecare[3], solutieOarecare[4] - 1]) < cost(solutieCurenta);
       assert false;
       
     }
-    else if(solutieOarecare[3] < solutieCurenta[3]+1)
+    else if(solutieOarecare[3] < solutieCurenta[3])
       {
-        assert (solutieOarecare[0]+(5*solutieOarecare[1])+(10*solutieOarecare[2]))>20;
+        assert (solutieOarecare[0] + (5 * solutieOarecare[1]) + (10 * solutieOarecare[2])) > 20;
         
-        if(solutieOarecare[2]>=2)
+        if(solutieOarecare[2] >= 2)
         {
-            var nouaSolutieOarecare := [solutieOarecare[0],solutieOarecare[1],solutieOarecare[2]-2,solutieOarecare[3]+1];
-            B(copie,nr,nouaSolutieOarecare, solutieCurenta);
+            assert solutieOarecare[2] >= 2;
+            var nouaSolutieOarecare := [solutieOarecare[0], solutieOarecare[1], solutieOarecare[2] - 2, solutieOarecare[3] + 1, solutieOarecare[4]];
+            exchangeArgumentCaz50(rest, suma, nouaSolutieOarecare, solutieCurenta);
         }
-        else if(solutieOarecare[2]>=1 && solutieOarecare[1]>=2)
+        else if(solutieOarecare[2] >= 1 && solutieOarecare[1] >= 2)
         {
-            var nouaSolutieOarecare := [solutieOarecare[0],solutieOarecare[1]-2,solutieOarecare[2]-1,solutieOarecare[3]+1];
-            B(copie,nr,nouaSolutieOarecare, solutieCurenta);
+            var nouaSolutieOarecare := [solutieOarecare[0], solutieOarecare[1] - 2, solutieOarecare[2] - 1, solutieOarecare[3] + 1, solutieOarecare[4]];
+            exchangeArgumentCaz50(rest, suma, nouaSolutieOarecare, solutieCurenta);
         }
-        else if(solutieOarecare[2]>=1 && solutieOarecare[1]>=1 && solutieOarecare[0]>=5)
+        else if(solutieOarecare[2] >= 1 && solutieOarecare[1] >= 1 && solutieOarecare[0] >= 5)
         {
-            var nouaSolutieOarecare := [solutieOarecare[0]-5,solutieOarecare[1]-1,solutieOarecare[2]-1,solutieOarecare[3]+1];
-            B(copie,nr,nouaSolutieOarecare, solutieCurenta);
+            var nouaSolutieOarecare := [solutieOarecare[0] - 5, solutieOarecare[1] - 1, solutieOarecare[2] - 1, solutieOarecare[3] + 1, solutieOarecare[4]];
+            exchangeArgumentCaz50(rest, suma, nouaSolutieOarecare, solutieCurenta);
         }
-        else if(solutieOarecare[1]>=4)
+        else if(solutieOarecare[1] >= 4)
         {
-            var nouaSolutieOarecare := [solutieOarecare[0],solutieOarecare[1]-4,solutieOarecare[2],solutieOarecare[3]+1];
-            B(copie,nr,nouaSolutieOarecare, solutieCurenta);
+            var nouaSolutieOarecare := [solutieOarecare[0], solutieOarecare[1] - 4, solutieOarecare[2], solutieOarecare[3] + 1, solutieOarecare[4]];
+            exchangeArgumentCaz50(rest, suma, nouaSolutieOarecare, solutieCurenta);
         }
-        else if(solutieOarecare[1]>=3 && solutieOarecare[0]>=5)
+        else if(solutieOarecare[1] >= 3 && solutieOarecare[0] >= 5)
         {
-            var nouaSolutieOarecare := [solutieOarecare[0]-5,solutieOarecare[1]-3,solutieOarecare[2],solutieOarecare[3]+1];
-            B(copie,nr,nouaSolutieOarecare, solutieCurenta);
+            var nouaSolutieOarecare := [solutieOarecare[0] - 5, solutieOarecare[1] - 3, solutieOarecare[2], solutieOarecare[3] + 1, solutieOarecare[4]];
+            exchangeArgumentCaz50(rest, suma, nouaSolutieOarecare, solutieCurenta);
         }
-        else if(solutieOarecare[1]>=2 && solutieOarecare[0]>=10)
+        else if(solutieOarecare[1] >= 2 && solutieOarecare[0] >= 10)
         {
-            var nouaSolutieOarecare := [solutieOarecare[0]-10,solutieOarecare[1]-2,solutieOarecare[2],solutieOarecare[3]+1];
-            B(copie,nr,nouaSolutieOarecare, solutieCurenta);
+            var nouaSolutieOarecare := [solutieOarecare[0] - 10, solutieOarecare[1] - 2, solutieOarecare[2], solutieOarecare[3] + 1, solutieOarecare[4]];
+            exchangeArgumentCaz50(rest, suma, nouaSolutieOarecare, solutieCurenta);
         }
-        else if(solutieOarecare[1]>=1 && solutieOarecare[0]>=15)
+        else if(solutieOarecare[1] >= 1 && solutieOarecare[0] >= 15)
         {
-          var nouaSolutieOarecare := [solutieOarecare[0]-15,solutieOarecare[1]-1,solutieOarecare[2],solutieOarecare[3]+1];
-            B(copie,nr,nouaSolutieOarecare, solutieCurenta);
+            var nouaSolutieOarecare := [solutieOarecare[0] - 15, solutieOarecare[1] - 1, solutieOarecare[2], solutieOarecare[3] + 1, solutieOarecare[4]];
+            exchangeArgumentCaz50(rest, suma, nouaSolutieOarecare, solutieCurenta);
         }
-        else if(solutieOarecare[0]>=20)
+        else if(solutieOarecare[0] >= 20)
         {
-            var nouaSolutieOarecare := [solutieOarecare[0]-20,solutieOarecare[1],solutieOarecare[2],solutieOarecare[3]+1];
-            B(copie,nr,nouaSolutieOarecare, solutieCurenta);
+            var nouaSolutieOarecare := [solutieOarecare[0] - 20, solutieOarecare[1], solutieOarecare[2], solutieOarecare[3] + 1, solutieOarecare[4]];
+            exchangeArgumentCaz50(rest, suma, nouaSolutieOarecare, solutieCurenta);
         }
-        else if(solutieOarecare[2]>=1 && solutieOarecare[0]>=10)
+        else if(solutieOarecare[2] >= 1 && solutieOarecare[0] >= 10)
         {
-            var nouaSolutieOarecare := [solutieOarecare[0]-10,solutieOarecare[1],solutieOarecare[2]-1,solutieOarecare[3]+1];
-            B(copie,nr,nouaSolutieOarecare, solutieCurenta);
+            var nouaSolutieOarecare := [solutieOarecare[0] - 10, solutieOarecare[1], solutieOarecare[2] - 1, solutieOarecare[3] + 1, solutieOarecare[4]];
+            exchangeArgumentCaz50(rest, suma, nouaSolutieOarecare, solutieCurenta);
         }
       }
 
-    assert solutieOarecare[3] == (solutieCurenta[3]+1);
+    assert solutieOarecare[3] == solutieCurenta[3];
 
-    if(solutieOarecare[2]>solutieCurenta[2])
+    if(solutieOarecare[2] > solutieCurenta[2])
     {
-      assert cost([solutieOarecare[0],solutieOarecare[1],solutieOarecare[2],solutieOarecare[3]-1]) < cost(solutieCurenta);
+      assert cost([solutieOarecare[0], solutieOarecare[1], solutieOarecare[2], solutieOarecare[3], solutieOarecare[4] - 1]) < cost(solutieCurenta);
       assert false;
     }
     else if(solutieOarecare[2] < solutieCurenta[2])
       {
-        assert (solutieOarecare[0]+(5*solutieOarecare[1]))>10;
+        assert (solutieOarecare[0] + (5 * solutieOarecare[1])) > 10;
 
-        if(solutieOarecare[0]>=10)
+        if(solutieOarecare[0] >= 10)
         {
-          var nouaSolutieOarecare := [solutieOarecare[0]-10,solutieOarecare[1],solutieOarecare[2]+1,solutieOarecare[3]];
-          B(copie,nr,nouaSolutieOarecare, solutieCurenta);
+          var nouaSolutieOarecare := [solutieOarecare[0] - 10, solutieOarecare[1], solutieOarecare[2] + 1, solutieOarecare[3], solutieOarecare[4]];
+          exchangeArgumentCaz50(rest, suma, nouaSolutieOarecare, solutieCurenta);
         }
-        else if(solutieOarecare[1]>=2){
-            var nouaSolutieOarecare := [solutieOarecare[0],solutieOarecare[1]-2,solutieOarecare[2]+1,solutieOarecare[3]];
-             B(copie,nr,nouaSolutieOarecare, solutieCurenta);
+        else if(solutieOarecare[1] >= 2){
+            var nouaSolutieOarecare := [solutieOarecare[0], solutieOarecare[1] - 2, solutieOarecare[2] + 1, solutieOarecare[3], solutieOarecare[4]];
+            exchangeArgumentCaz50(rest, suma, nouaSolutieOarecare, solutieCurenta);
         }
           else
           {
-            var nouaSolutieOarecare := [solutieOarecare[0]-5,solutieOarecare[1]-1,solutieOarecare[2]+1,solutieOarecare[3]];
-             B(copie,nr,nouaSolutieOarecare, solutieCurenta);
+            var nouaSolutieOarecare := [solutieOarecare[0] - 5, solutieOarecare[1] - 1, solutieOarecare[2] + 1, solutieOarecare[3], solutieOarecare[4]];
+            exchangeArgumentCaz50(rest, suma, nouaSolutieOarecare, solutieCurenta);
           }
         }
         assert solutieOarecare[2] == solutieCurenta[2];
 
-      if(solutieOarecare[1]>solutieCurenta[1])
+      if(solutieOarecare[1] > solutieCurenta[1])
     {
-      assert cost([solutieOarecare[0],solutieOarecare[1],solutieOarecare[2],solutieOarecare[3]-1]) < cost(solutieCurenta);
+      assert cost([solutieOarecare[0], solutieOarecare[1], solutieOarecare[2], solutieOarecare[3], solutieOarecare[4] - 1]) < cost(solutieCurenta);
       assert false;
     }
     else
     {
-      if(solutieOarecare[1]<solutieCurenta[1])
+      if(solutieOarecare[1] < solutieCurenta[1])
       {
-        assert solutieOarecare[0]>=5;
-      
-          var nouaSolutieOarecare := [solutieOarecare[0]-5,solutieOarecare[1]+1,solutieOarecare[2],solutieOarecare[3]];
-          B(copie, nr, nouaSolutieOarecare, solutieCurenta);
+          assert solutieOarecare[0] >= 5;
+          var nouaSolutieOarecare := [solutieOarecare[0] - 5, solutieOarecare[1] + 1, solutieOarecare[2], solutieOarecare[3], solutieOarecare[4]];
+          exchangeArgumentCaz50(rest, suma, nouaSolutieOarecare, solutieCurenta);
         
       }
     }
-    assert solutieOarecare[0]==solutieCurenta[0];
+    assert solutieOarecare[0] == solutieCurenta[0];
     assert false;
 
   }
 }
 
-lemma esteSolutiePentruCopie(copie:int,nr: int, solutieCurenta:seq<int>)
+lemma solutieCurentaAreCostMinim(rest : int, suma : int, solutieCurenta : seq<int>)
   requires esteSolutieValida(solutieCurenta)
-  requires copie >= 20
-  requires esteSolutie(solutieCurenta,copie-20)
-  requires esteSolutieOptima(solutieCurenta,copie-20)
-  ensures esteSolutieOptima([solutieCurenta[0],solutieCurenta[1],solutieCurenta[2],1+solutieCurenta[3]],copie)
+  requires rest >= 50
+  requires esteSolutie(solutieCurenta, rest - 50)
+  requires esteSolutieOptima(solutieCurenta, rest - 50)
+  ensures esteSolutieOptima([solutieCurenta[0], solutieCurenta[1], solutieCurenta[2], solutieCurenta[3], 1 + solutieCurenta[4]], rest)
 {
-  forall solutieOarecare | esteSolutieValida(solutieOarecare) && esteSolutie(solutieOarecare,copie)
-    ensures cost(solutieOarecare)>=cost([solutieCurenta[0],solutieCurenta[1],solutieCurenta[2],1+solutieCurenta[3]])
+  forall solutieOarecare | esteSolutieValida(solutieOarecare) && esteSolutie(solutieOarecare, rest)
+    ensures cost(solutieOarecare) >= cost([solutieCurenta[0], solutieCurenta[1], solutieCurenta[2], solutieCurenta[3], 1 + solutieCurenta[4]])
   {
-    B(copie,nr, solutieOarecare, solutieCurenta);
+    exchangeArgumentCaz50(rest, suma, solutieOarecare, solutieCurenta);
   }
   
 }
 
-lemma aux(copie: int ,nr: int, solutieOarecare : seq<int>, solutieFinala : seq<int>, solutieCurenta:seq<int>)
+
+lemma solutieFianalaAreCostMinim(rest : int, suma : int, solutieOarecare : seq<int>, solutieFinala : seq<int>, solutieCurenta : seq<int>)
   requires esteSolutieValida(solutieOarecare)
   requires esteSolutieValida(solutieFinala)
   requires esteSolutieValida(solutieCurenta)
-  requires copie >= 20
-  requires esteSolutieOptima(solutieCurenta,copie-20)
-  requires esteSolutie([solutieFinala[0]+solutieCurenta[0],solutieFinala[1]+solutieCurenta[1],solutieFinala[2]+solutieCurenta[2],1+solutieFinala[3]+solutieCurenta[3]],nr)
-  requires esteSolutie(solutieOarecare,nr)
-  requires INV(copie,nr,solutieFinala)
-  ensures cost(solutieOarecare) >= cost([solutieFinala[0]+solutieCurenta[0],solutieFinala[1]+solutieCurenta[1],solutieFinala[2]+solutieCurenta[2],1+solutieFinala[3]+solutieCurenta[3]])
+  requires rest >= 50
+  requires esteSolutieOptima(solutieCurenta, rest - 50)
+  requires esteSolutie([solutieFinala[0] + solutieCurenta[0], solutieFinala[1] + solutieCurenta[1], solutieFinala[2] + solutieCurenta[2], solutieFinala[3] + solutieCurenta[3], 1 + solutieFinala[4] + solutieCurenta[4]], suma)
+  requires esteSolutie(solutieOarecare, suma)
+  requires INV(rest, suma, solutieFinala)
+  ensures cost(solutieOarecare) >= cost([solutieFinala[0] + solutieCurenta[0], solutieFinala[1] + solutieCurenta[1], solutieFinala[2] + solutieCurenta[2], solutieFinala[3] + solutieCurenta[3], 1 + solutieFinala[4] + solutieCurenta[4]])
 {
-  esteSolutiePentruCopie(copie,nr,solutieCurenta);
+  solutieCurentaAreCostMinim(rest, suma, solutieCurenta);
 }
 
 
 
 
-lemma cazMaxim20(copie: int,nr: int, solutieFinala : seq<int>)
-  requires copie >= 20
+lemma cazMaxim50(rest : int, suma : int, solutieFinala : seq<int>)
+  requires rest >= 50
   requires esteSolutieValida(solutieFinala)
-  requires INV(copie,nr,solutieFinala)
-  ensures INV(copie-20,nr,[solutieFinala[0],solutieFinala[1],solutieFinala[2],solutieFinala[3]+1])
+  requires INV(rest, suma, solutieFinala)
+  ensures INV(rest - 50, suma, [solutieFinala[0], solutieFinala[1], solutieFinala[2], solutieFinala[3], 1 + solutieFinala[4]])
 {
   assert forall solutieCurenta :: esteSolutieValida(solutieCurenta) ==>
-          (esteSolutie(solutieCurenta,copie) ==> 
-          esteSolutie([solutieFinala[0]+solutieCurenta[0],solutieFinala[1]+solutieCurenta[1],solutieFinala[2]+solutieCurenta[2],solutieFinala[3]+solutieCurenta[3]],nr));
+          (esteSolutie(solutieCurenta, rest) ==> 
+          esteSolutie([solutieFinala[0] + solutieCurenta[0], solutieFinala[1] + solutieCurenta[1], solutieFinala[2] + solutieCurenta[2],
+           solutieFinala[3] + solutieCurenta[3],solutieFinala[4] + solutieCurenta[4]], suma));
 
    forall solutieCurenta | esteSolutieValida(solutieCurenta) 
-          && esteSolutie(solutieCurenta,copie-20) 
-          ensures esteSolutie([solutieFinala[0]+solutieCurenta[0],solutieFinala[1]+solutieCurenta[1],solutieFinala[2]+solutieCurenta[2],solutieFinala[3]+solutieCurenta[3]+1],nr)
+          && esteSolutie(solutieCurenta, rest - 50) 
+          ensures esteSolutie([solutieFinala[0] + solutieCurenta[0], solutieFinala[1] + solutieCurenta[1], solutieFinala[2] + solutieCurenta[2], 
+          solutieFinala[3] + solutieCurenta[3], 1 + solutieFinala[4] + solutieCurenta[4]], suma)
    {
-     assert esteSolutie([solutieCurenta[0],solutieCurenta[1],solutieCurenta[2],solutieCurenta[3]+1],copie);
+     assert esteSolutie([solutieCurenta[0], solutieCurenta[1], solutieCurenta[2], solutieCurenta[3], 1 + solutieCurenta[4]], rest);
    }
   
 
   forall solutieCurenta | esteSolutieValida(solutieCurenta) 
-          && esteSolutieOptima(solutieCurenta,copie-20) 
-          ensures esteSolutieOptima([solutieFinala[0]+solutieCurenta[0],solutieFinala[1]+solutieCurenta[1],solutieFinala[2]+solutieCurenta[2],solutieFinala[3]+solutieCurenta[3]+1],nr)
+          && esteSolutieOptima(solutieCurenta, rest - 50) 
+          ensures esteSolutieOptima([solutieFinala[0] + solutieCurenta[0], solutieFinala[1] + solutieCurenta[1], solutieFinala[2] + solutieCurenta[2],
+           solutieFinala[3] + solutieCurenta[3], 1 + solutieFinala[4] + solutieCurenta[4]], suma)
   {
 
-    assert esteSolutie(solutieCurenta,copie-20);
-    assert esteSolutie([solutieCurenta[0],solutieCurenta[1],solutieCurenta[2],solutieCurenta[3]+1],copie);
+    assert esteSolutie(solutieCurenta, rest - 50);
+    assert esteSolutie([solutieCurenta[0], solutieCurenta[1], solutieCurenta[2], solutieCurenta[3], 1 + solutieCurenta[4]], rest);
 
     assert forall solutieOarecare :: esteSolutieValida(solutieOarecare)
-          && esteSolutie(solutieOarecare,copie-20) 
+          && esteSolutie(solutieOarecare, rest - 50) 
           ==> cost(solutieOarecare) >= cost(solutieCurenta);
 
 
-    assert esteSolutie([solutieFinala[0]+solutieCurenta[0],solutieFinala[1]+solutieCurenta[1],solutieFinala[2]+solutieCurenta[2],solutieFinala[3]+solutieCurenta[3]+1],nr);
+    assert esteSolutie([solutieFinala[0] + solutieCurenta[0], solutieFinala[1] + solutieCurenta[1], solutieFinala[2] + solutieCurenta[2], 
+      solutieFinala[3] + solutieCurenta[3], 1 + solutieFinala[4] + solutieCurenta[4]], suma);
 
     forall solutieOarecare | esteSolutieValida(solutieOarecare)
-                 && esteSolutie(solutieOarecare,nr)
-      ensures cost(solutieOarecare) >= cost([solutieFinala[0]+solutieCurenta[0],solutieFinala[1]+solutieCurenta[1],solutieFinala[2]+solutieCurenta[2],1+solutieFinala[3]+solutieCurenta[3]])
+                 && esteSolutie(solutieOarecare, suma)
+      ensures cost(solutieOarecare) >= cost([solutieFinala[0] + solutieCurenta[0], solutieFinala[1] + solutieCurenta[1], solutieFinala[2] + solutieCurenta[2], solutieFinala[3] + solutieCurenta[3], 1 + solutieFinala[4] + solutieCurenta[4]])
       {
-          aux(copie, nr, solutieOarecare, solutieFinala, solutieCurenta);
+          solutieFianalaAreCostMinim(rest, suma, solutieOarecare, solutieFinala, solutieCurenta);
       }
 
     assert forall solutieOarecare :: esteSolutieValida(solutieOarecare)
-             && esteSolutie(solutieOarecare,nr) 
-          ==> cost(solutieOarecare) >= cost([solutieFinala[0]+solutieCurenta[0],solutieFinala[1]+solutieCurenta[1],solutieFinala[2]+solutieCurenta[2],1+solutieFinala[3]+solutieCurenta[3]]);
+             && esteSolutie(solutieOarecare, suma) 
+          ==> cost(solutieOarecare) >= cost([solutieFinala[0] + solutieCurenta[0], solutieFinala[1] + solutieCurenta[1], solutieFinala[2] + solutieCurenta[2], solutieFinala[3] + solutieCurenta[3], 1 + solutieFinala[4] + solutieCurenta[4]]);
   }
 
 
   assert forall solutieCurenta :: esteSolutieValida(solutieCurenta)
-          && esteSolutieOptima(solutieCurenta,copie-20) ==> 
-          esteSolutieOptima([solutieFinala[0]+solutieCurenta[0],solutieFinala[1]+solutieCurenta[1],solutieFinala[2]+solutieCurenta[2],1+solutieFinala[3]+solutieCurenta[3]],nr);
+          && esteSolutieOptima(solutieCurenta, rest - 50) ==> 
+          esteSolutieOptima([solutieFinala[0] + solutieCurenta[0], solutieFinala[1] + solutieCurenta[1], solutieFinala[2] + solutieCurenta[2],
+           solutieFinala[3] + solutieCurenta[3], 1 + solutieFinala[4] + solutieCurenta[4]], suma);
 
 
   assert forall solutieCurenta :: esteSolutieValida(solutieCurenta) ==>
-          (esteSolutie(solutieCurenta,copie-20) ==> 
-          esteSolutie([solutieFinala[0]+solutieCurenta[0],solutieFinala[1]+solutieCurenta[1],solutieFinala[2]+solutieCurenta[2],1+solutieFinala[3]+solutieCurenta[3]],nr));
+          (esteSolutie(solutieCurenta, rest - 50) ==> 
+          esteSolutie([solutieFinala[0] + solutieCurenta[0], solutieFinala[1] + solutieCurenta[1], solutieFinala[2] + solutieCurenta[2], 
+          solutieFinala[3] + solutieCurenta[3], 1 + solutieFinala[4] + solutieCurenta[4]], suma));
   
   assert forall solutieCurenta :: esteSolutieValida(solutieCurenta) ==>        
-          (esteSolutieOptima(solutieCurenta,copie-20) ==> 
-          esteSolutieOptima([solutieFinala[0]+solutieCurenta[0],solutieFinala[1]+solutieCurenta[1],solutieFinala[2]+solutieCurenta[2],solutieFinala[3]+solutieCurenta[3]+1],nr));
+          (esteSolutieOptima(solutieCurenta, rest - 50) ==> 
+          esteSolutieOptima([solutieFinala[0] + solutieCurenta[0], solutieFinala[1] + solutieCurenta[1], solutieFinala[2] + solutieCurenta[2],
+           solutieFinala[3] + solutieCurenta[3], 1 + solutieFinala[4] + solutieCurenta[4]], suma));
 
-  assert  INV(copie-20,nr,[solutieFinala[0],solutieFinala[1],solutieFinala[2],1+solutieFinala[3]]);
+  assert  INV(rest - 50, suma, [solutieFinala[0], solutieFinala[1], solutieFinala[2], solutieFinala[3], 1 + solutieFinala[4]]);
 }
 
 
 
-  method nrMinimBancnote(nr: int) returns (solutie: seq<int>)
-    requires nr>=0
+  method nrMinimBancnote(suma : int) returns (solutie : seq<int>)
+    requires suma >= 0
     ensures esteSolutieValida(solutie)
-    ensures esteSolutie(solutie,nr)
-    ensures esteSolutieOptima(solutie,nr)
+    ensures esteSolutie(solutie, suma)
+    ensures esteSolutieOptima(solutie, suma)
 {
 
-    var copie:=  nr;
+    var rest  :=  suma;
     var s1 := 0;
     var s5 := 0;
     var s10 := 0;
     var s20 := 0;
-    while(copie > 0)
-      decreases copie
-      invariant 0<=copie<=nr
-      invariant esteSolutie([s1,s5,s10,s20],nr-copie)
-      invariant INV(copie,nr,[s1,s5,s10,s20])
+    var s50 := 0;
+    while(rest > 0)
+      decreases rest
+      invariant 0 <= rest <= suma
+      invariant esteSolutie([s1, s5, s10, s20, s50], suma - rest)
+      invariant INV(rest, suma, [s1, s5, s10, s20, s50])
     {
         var i := 0;
-        var s := gasireMaxim(copie);
+        var s := gasireMaxim(rest);
         if( s == 1){
-            cazMaxim1(copie,nr,[s1,s5,s10,s20]);
-            s1:=s1+1;
-            assert esteSolutie([s1,s5,s10,s20],nr-(copie-1));
-            assert INV(copie-1,nr,[s1,s5,s10,s20]);
+            cazMaxim1(rest, suma, [s1, s5, s10, s20, s50]);
+            s1 := s1 + 1;
+            assert esteSolutie([s1, s5, s10, s20, s50], suma - (rest - 1));
+            assert INV(rest - 1, suma, [s1, s5, s10, s20, s50]);
         }
         else if(s == 5)
             {
-                cazMaxim5(copie,nr,[s1,s5,s10,s20]);
-                s5:=s5+1;
-                assert esteSolutie([s1,s5,s10,s20],nr-(copie-5));
-                assert INV(copie-5,nr,[s1,s5,s10,s20]);
+                cazMaxim5(rest, suma, [s1, s5, s10, s20, s50]);
+                s5 := s5 + 1;
+                assert esteSolutie([s1, s5, s10, s20, s50], suma - (rest - 5));
+                assert INV(rest - 5, suma, [s1, s5, s10, s20, s50]);
 
             }
             else if (s == 10){
-                cazMaxim10(copie,nr,[s1,s5,s10,s20]);
-                s10:=s10+1;
-                assert esteSolutie([s1,s5,s10,s20],nr-(copie-10));
-                assert INV(copie-10,nr,[s1,s5,s10,s20]);
+                cazMaxim10(rest, suma, [s1, s5, s10, s20, s50]);
+                s10 := s10 + 1;
+                assert esteSolutie([s1, s5, s10, s20, s50], suma - (rest - 10));
+                assert INV(rest - 10, suma, [s1, s5, s10, s20, s50]);
 
+            }
+            else if(s == 20){
+                cazMaxim20(rest, suma, [s1, s5, s10, s20, s50]);
+                s20 := s20 + 1;
+                assert esteSolutie([s1, s5, s10, s20, s50], suma - (rest - 20));
+                assert INV(rest - 20, suma, [s1, s5, s10, s20, s50]);
             }
             else{
-                cazMaxim20(copie,nr,[s1,s5,s10,s20]);
-                s20:=s20+1;
-                assert esteSolutie([s1,s5,s10,s20],nr-(copie-20));
-                assert INV(copie-20,nr,[s1,s5,s10,s20]);
+                cazMaxim50(rest, suma, [s1, s5, s10, s20, s50]);
+                s50 := s50 + 1;
+                assert esteSolutie([s1, s5, s10, s20, s50], suma - (rest - 50));
+                assert INV(rest - 50, suma, [s1, s5, s10, s20, s50]);
             }
 
-        copie := copie-s;
+        rest := rest - s;
     }
-    solutie := [s1,s5,s10,s20];
+    solutie := [s1, s5, s10, s20, s50];
 }
 
 
 method Main() {
-  var nr:= 58;
-  var sol:=nrMinimBancnote(nr);
-  print sol;
+  var suma := 188;
+  var solutie := nrMinimBancnote(suma);
+  print "Solutia este = ";
+  print "1: ";
+  print solutie[0];
+  print ", ";
+  print "5: ";
+  print solutie[1];
+  print ", ";
+  print "10: ";
+  print solutie[2];
+  print ", ";
+  print "20: ";
+  print solutie[3];
+  print ", ";
+  print "50: ";
+  print solutie[4];
 }
